Lerchner/test.thy
@@ -1,151 +1,76 @@
 theory test
-  imports Main HOL.List DFA_to_RegExp
+  imports Main HOL.List DFA_to_RegExp2
 begin
 
-locale dfa =
-  fixes n :: nat
-  and sigma :: "'a list"
-  and nxt :: "nat \<Rightarrow> 'a \<Rightarrow> nat"
-  and Fin :: "nat set"
-begin
-  
-fun nxts :: "'a list \<Rightarrow> nat \<Rightarrow> nat" where
-  "nxts [] q = q" |
-  "nxts (a#w) q = nxts w (nxt q a)"
-  
-definition accepted :: "'a list \<Rightarrow> bool" where
-  "accepted w = (nxts w 0 \<in> Fin)"
-
-fun list_to_rexp :: "'a list \<Rightarrow> 'a rexp" where
-  "list_to_rexp [] = Zero" |
-  "list_to_rexp [x] = Atom x" |
-  "list_to_rexp (x#xs) = Plus (Atom x) (list_to_rexp xs)"
-
-definition arc :: "nat \<Rightarrow> nat \<Rightarrow> 'a rexp" where
-  "arc i j = list_to_rexp [a \<leftarrow> sigma. nxt i a = j]"
-
-(* Test instance *)
-definition test_sigma :: "string list"
-where "test_sigma = [''a'', ''b'']"
-
-fun test_nxt :: "nat \<Rightarrow> string \<Rightarrow> nat" where
-  "test_nxt 0 ''a'' = 1" |
-  "test_nxt 0 ''b'' = 0" |
-  "test_nxt (Suc 0) ''a'' = 1" |
-  "test_nxt (Suc 0) ''b'' = 0"
-
-definition test_Fin :: "nat set"
-where "test_Fin = {1}"
-
-(* Test cases *)
-lemma "arc 0 1 = list_to_rexp [''a'']"
-  by (simp add: arc_def test_sigma_def)
-
-lemma "arc 0 0 = list_to_rexp [''b'']"
-  by (simp add: arc_def test_sigma_def)
-
-lemma "arc 1 1 = list_to_rexp [''a'']"
-  by (simp add: arc_def test_sigma_def)
-
-end
-
-end
-
-
-lemma start_exist: "1 \<in> S"
-   by (metis atLeastAtMost_iff dfa_axioms dfa_def leI less_one not_gr_zero)
-
-
-fun nxts :: "'a list \<Rightarrow> nat \<Rightarrow> nat" where
-  "nxts [] q = q" |
-  "nxts (a#w) q = nxts w (nxt q a)"
-  
-definition accepted :: "'a list \<Rightarrow> bool" where
-  "accepted w = (nxts w 1 \<in> Fin)"
-
-definition word_run_from_i_j :: "'a list \<Rightarrow> nat \<Rightarrow> nat \<Rightarrow> bool" where
-  "word_run_from_i_j w i j =  (nxts w i = j)"
-
-
-corollary accepted_run:"accepted xs = (\<exists>j\<in> Fin. word_run_from_i_j xs 1 j) "
-  by (simp add: accepted_def word_run_from_i_j_def)
-
-(* Your work goes here: *)
-
-
-
-
-(** The traversed states of a word w. **)
-fun path_of_word :: "'a list \<Rightarrow> nat  \<Rightarrow> nat list" where
-  "path_of_word [] i = [i]" |
-  "path_of_word (a#w) i = i # path_of_word w (nxt i a) "
-
-lemma path_in_S:"i \<in> S \<Longrightarrow> set (path_of_word w i) \<subseteq> S"
-  apply(induction w arbitrary: i)
-  apply(auto)
-  by (meson in_mono transitions_in_S)
-
-
-
-fun intermediate_path:: "nat list \<Rightarrow> nat list" where
-  "intermediate_path p = butlast (tl p)"
-
-lemma intermediate_effect:"intermediate_path (a # is @ [e]) = is"
-  by simp
-
-definition paths_between :: "nat \<Rightarrow> nat  \<Rightarrow> (nat list) set" where
-  "paths_between i j = {path_of_word w i | w . word_run_from_i_j w i j}"
-
-(** The intermediate path consists of all nodes except the first and last nodes. **)
-definition intermediate_path_restricted :: "nat list \<Rightarrow> nat  \<Rightarrow> bool" where
-  "intermediate_path_restricted p k = (\<forall>s. s \<in> set (intermediate_path p) \<longrightarrow> s \<le> k)"
-
-
-(** A path is restricted to a node k if no intermediate node in the path is greater than k. **)
-definition restricetd_paths_between :: "nat \<Rightarrow> nat \<Rightarrow> nat \<Rightarrow> (nat list) set" where
-  "restricetd_paths_between i j k = {p. p \<in> paths_between i j \<and> intermediate_path_restricted p k}"
-
-
-corollary path_word_restricted_n:"i \<in> S \<Longrightarrow> j \<in> S  \<Longrightarrow>paths_between i j = restricetd_paths_between i j n"
-  unfolding restricetd_paths_between_def paths_between_def intermediate_path_restricted_def
-  apply(auto)
-  by (metis atLeastAtMost_iff in_mono in_set_butlastD list.sel(2) list.set_sel(2) path_in_S state_set_def)
-
-
-lemma intermediate_smaller: "set (intermediate_path p) \<subseteq> set p"
-  apply(auto)
-  by (metis in_set_butlastD list.sel(2) list.set_sel(2))
-
-corollary restricted_n:"i\<in> S \<Longrightarrow> intermediate_path_restricted (path_of_word w i) n"
-  unfolding intermediate_path_restricted_def
-  by (metis atLeastAtMost_iff in_mono intermediate_smaller path_in_S state_set_def)
+interpretation simple_dfa: dfa 
+  2 (* Number of states *)
+  "{1, 2}" (* Set of states *)
+  "[0::nat,1]" (* Alphabet *)
+  "\<lambda>i a. if i = 1 then (if a = 1 then 1 else 2) else 2 " (* Transition function *)
+  "{2}" (* Set of accepting states *)
+proof 
+  show "(0::nat) < 2"
+    by simp  
+next
+  show "{1::nat, 2} = {1..2}"
+    by (metis Icc_eq_insert_lb_nat Suc_1 atLeastAtMost_singleton lessI less_or_eq_imp_le)
+next
+  show "\<And>i a. i \<in> {1::nat, 2} \<longrightarrow> (if i = 1 then if a = 1 then 1 else 2 else 2) \<in> {1::nat, 2}"
+    by(auto)
+next
+  show "{2} \<subseteq> {1, 2}"
+    by auto
+next 
+  show" \<And>i a. i \<in> {1, 2} \<Longrightarrow> a \<in> set [0, 1] \<Longrightarrow> (if i = 1 then if a = 1 then 1 else 2 else 2) \<in> {1, 2}"
+    by auto
+qed 
  
 
-(** somehow this is necessery for automation **)
-lemma x:"\<Union>{lang x | x. x \<in> set (map A xs)} = \<Union>{ lang (A x) | x. x \<in> set (xs)} "
-  by auto
-
-lemma path_restricted_mono:"intermediate_path_restricted xs k \<Longrightarrow> intermediate_path_restricted xs (k+1)"
-  unfolding intermediate_path_restricted_def
-  apply(auto)
-  done
 
 
-  
+fun arcs_rexp :: "nat \<Rightarrow> nat \<Rightarrow> nat rexp" where
+  "arcs_rexp i j =  List.foldr Plus 
+                  (List.map Atom [ a \<leftarrow> [0::nat,1].  (if i = 1 then (if a = 1 then 1 else 2) else 2)= j ]) 
+              Zero"
+
+
+fun R :: "nat \<Rightarrow> nat \<Rightarrow> nat \<Rightarrow> nat rexp " where
+  "R i j 0 = (if i \<noteq> j then arcs_rexp i j else Plus One (arcs_rexp i j))" |
+  "R i j (Suc k) = ( 
+                   (  let R'= R    i       j    k in
+                      let u = R    i    (Suc k) k in
+                      let v = R (Suc k) (Suc k) k in
+                      let w = R (Suc k)    j    k in
+                    Plus  R' (Times u (Times (Star v) w))))"
+
+
+fun simp_rexp:: "nat rexp \<Rightarrow> nat rexp" where
+   "simp_rexp (Plus a Zero) = a" |
+   "simp_rexp (Plus Zero a) = a" |
+   "simp_rexp (Plus a b) = Plus (simp_rexp a) (simp_rexp b)" |
+   "simp_rexp (Times Zero b) =  Zero"|
+   "simp_rexp (Times a Zero) =  Zero"|
+   "simp_rexp (Times a b) = ( Times (simp_rexp a) (simp_rexp b))"|
+   "simp_rexp (Star (Plus a One)) =  (Star (simp_rexp a))"|
+   "simp_rexp (Star (Plus One b)) =  (Star (simp_rexp b))"|
+   "simp_rexp (Star x) =  (Star (simp_rexp x))"|
+   "simp_rexp x = x"
  
-(** Util **)
+   
+ 
+value "simp_rexp (R 1 1 0) "
+value "simp_rexp (R 1 2 0) "
+value "simp_rexp (R 2 1 0) "
+value "simp_rexp (R 2 2 0) "
 
-lemma accepted_path_k:"word_run_from_i_j w k j = (last (path_of_word w k) = j)"
-  apply(induction w k rule: path_of_word.induct)
-  apply(auto simp add:word_run_from_i_j_def)
-  using dfa.path_of_word.elims dfa_axioms apply blast
-  using dfa.path_of_word.elims dfa_axioms by blast
+value "simp_rexp (simp_rexp (simp_rexp (R 1 1 1)))"
+value "simp_rexp (simp_rexp (simp_rexp (R 1 2 1)))"
+value "simp_rexp (simp_rexp (simp_rexp (R 2 1 1)))"
+value "simp_rexp (simp_rexp (simp_rexp (R 2 2 1)))"
 
-corollary accepted_path:"accepted w  = (\<exists>j \<in> Fin. word_run_from_i_j w 1 j)"
-  unfolding accepted_def word_run_from_i_j_def
-  by(auto)
-
-
-
+value "simp_rexp (R 1 1 2) "
+value "simp_rexp (simp_rexp (simp_rexp (simp_rexp (simp_rexp  (R 1 2 2) ))))"
+value "simp_rexp (simp_rexp (simp_rexp (simp_rexp (simp_rexp  (R 2 1 2) ))))"
+value "simp_rexp (simp_rexp (simp_rexp (simp_rexp (simp_rexp  (R 2 2 2) ))))"
 
 end
