Lerchner/DFA_to_RegExp2.thy
@@ -20,19 +20,23 @@ definition arcs_rexp :: "nat \<Rightarrow> nat \<Rightarrow> 'a rexp" where
    "arcs_rexp i j = foldr Plus [Atom a . a \<leftarrow> sigma, nxt i a = j] Zero"
 
 
+
 (** todo start at -1?**)
-fun R:: "nat \<Rightarrow> nat \<Rightarrow> nat \<Rightarrow> 'a rexp " where
-  "R i j 0 = (if i \<noteq> j then arcs_rexp i j else Plus One (arcs_rexp i j))" |
-  "R i j (Suc k) = (  let R'= R    i       j    k in
+fun R :: "nat \<Rightarrow> nat \<Rightarrow> nat \<Rightarrow> 'a rexp " where
+  "R i j 0 = (if i \<notin> S \<or> j \<notin> S then Zero else 
+               (if i \<noteq> j then arcs_rexp i j else Plus One (arcs_rexp i j)))" |
+  "R i j (Suc k) = (if i \<notin> S \<or> j \<notin> S then Zero else 
+                   (  let R'= R    i       j    k in
                       let u = R    i    (Suc k) k in
                       let v = R (Suc k) (Suc k) k in
                       let w = R (Suc k)    j    k in
-                    Plus  R' (Times u (Times (Star v) w)))"
+                    Plus  R' (Times u (Times (Star v) w))))"
 
 
+ 
 
 
-lemma lang_arcs_rexp:" lang (arcs_rexp i j) = { [a] | a.  nxt i a = j}"
+lemma lang_arcs_rexp:" lang (arcs_rexp i j) = { [a] | a. a \<in> set sigma \<and>  nxt i a = j}"
 proof -
     have " lang (arcs_rexp i j) = lang (foldr Plus [Atom a . a \<leftarrow> sigma, nxt i a = j] Zero)"
       by (simp add: arcs_rexp_def)
@@ -44,55 +48,90 @@ proof -
       by blast
     also have "... =  { [a] | a. a \<in> set sigma \<and> nxt i a = j}"
       by(auto)
-    also have "... =  { [a] | a.  nxt i a = j}"
-      by (simp add: transitions_valid)
     finally show ?thesis 
       by auto
-  qed
+qed
+
 
 lemma Rmono: "lang (R i j k) \<subseteq> lang (R i j (k + 1))"
-  by(auto)
+  apply(induction  i j k rule:R.induct)
+   apply(auto)
+  done
 
-lemma lang_Rij0:" lang (R i j 0) = { [a] | a.  nxt i a = j}  \<union> (if i = j then {[]} else {})"
+
+
+lemma lang_Rij0:"lang (R i j 0) = (if i\<notin> S \<or> j \<notin> S then {} 
+                                   else { [a] | a. a \<in> set sigma \<and>  nxt i a = j}  \<union> (if i = j then {[]} else {}))"
    by (simp add: lang_arcs_rexp)
+
+
+
+lemma R_valid_path:"w\<in> lang (R i j k) \<Longrightarrow> i \<in> S \<and> j \<in> S"
+  apply(induction i j k rule:R.induct)
+  apply (metis empty_iff lang_Rij0)
+  apply(auto)
+  apply (smt (verit, ccfv_threshold) empty_iff lang.simps(1))
+  by (smt (verit, best) all_not_in_conv lang.simps(1))
+
+
 
 
 lemma path_Rij0:" w\<in> lang (R i j 0) \<Longrightarrow> path_of_word w i = (if w=[] then [i] else [i,j])"
 proof -
   assume "w\<in> lang (R i j 0)"
-  then have "w \<in> { [a] | a.  nxt i a = j}  \<union> (if i = j then {[]} else {})"
-    using lang_Rij0 by fastforce
+  then have "w \<in> { [a] | a. a \<in> set sigma \<and>  nxt i a = j}  \<union> (if i = j then {[]} else {})"
+    by (metis (no_types, lifting) lang_Rij0 R_valid_path)
   then show "path_of_word w i = (if w=[] then [i] else [i,j])"
     apply(cases "i=j")
     by(auto)
 qed
 
 
-lemma no_intermediate_path_k0:"i \<in> S\<Longrightarrow> p = (path_of_word w i) \<Longrightarrow>  intermediate_path_restricted p 0 \<Longrightarrow> intermediate_path p = [] "
+lemma no_intermediate_path_k0:"i \<in> S \<Longrightarrow>  p = (path_of_word w i) \<Longrightarrow>  intermediate_path_restricted p 0 \<Longrightarrow> intermediate_path p = [] "
   unfolding  intermediate_path_restricted_def
-  by (metis atLeastAtMost_iff dual_order.trans intermediate_smaller list.exhaust list.set_intros(1) not_one_le_zero path_in_S state_set_def subset_iff)
-
-lemma path_shape_no_intermediate:"i \<in> S \<Longrightarrow> intermediate_path (path_of_word w i) = [] \<Longrightarrow> path_of_word w i = (if w=[] then [i] else [i,nxt i (hd w)])"
+  apply(induction w arbitrary:i)
+  apply(simp)
+  by (metis atLeastAtMost_iff intermediate_smaller le_zero_eq list.set_intros(1) neq_Nil_conv path_in_S state_set_def subset_iff zero_neq_one)
+ 
+lemma path_shape_no_intermediate:"intermediate_path (path_of_word w i) = [] \<Longrightarrow> path_of_word w i = (if w=[] then [i] else [i,nxt i (hd w)])"
   unfolding word_run_from_i_j_def
   apply(induction w arbitrary:i)
   apply(auto)
-  by (metis butlast.simps(2) butlast_tl list.discI list.sel(2) transitions_in_S)
+  by (metis butlast.simps(2) butlast_tl list.discI list.sel(2))
 
 lemma langR1j0_1:
   assumes "w \<in> lang (R i j 0)"
   shows "(word_run_from_i_j w i j \<and>  intermediate_path_restricted (path_of_word w i) 0)"
-  using assms unfolding word_run_from_i_j_def intermediate_path_restricted_def 
-  apply(cases "i=j")
-  by(auto simp add:lang_arcs_rexp)
+ proof -
+   have lang:"lang (R i j 0) =  { [a] | a. a \<in> set sigma \<and>  nxt i a = j}  \<union> (if i = j then {[]} else {})"
+     by (metis (no_types, lifting) assms lang_Rij0 R_valid_path)
 
+   have " i \<in> S "
+     using assms R_valid_path by blast
+
+   then have "word_run_from_i_j w i j"
+     apply(cases "i = j")
+     using lang assms word_run_from_i_j_def by force +
+
+   have "intermediate_path (path_of_word w i) = [] "
+     using assms path_Rij0 by force
+
+   then have "intermediate_path_restricted (path_of_word w i) 0"
+     unfolding intermediate_path_restricted_def
+     by simp
+  
+   then show ?thesis
+     by (simp add: \<open>word_run_from_i_j w i j\<close>)
+ qed
+
+ 
 lemma langR1j0_2:
-  assumes "i \<in> S"
-  and "word_run_from_i_j w i j" and "intermediate_path_restricted (path_of_word w i) 0"
+  assumes "word_run_from_i_j w i j" and "intermediate_path_restricted (path_of_word w i) 0"
   shows "w \<in> lang (R i j 0)"
 using assms proof -
    have "intermediate_path (path_of_word w i) = []"
-    using assms no_intermediate_path_k0 by auto
-
+     using assms(1) assms(2) no_intermediate_path_k0 word_run_sound by blast
+ 
   then have "path_of_word w i  =(if w=[] then [i] else [i,nxt i (hd w)])"
     using assms path_shape_no_intermediate by auto
 
@@ -103,9 +142,11 @@ using assms proof -
     by meson
   then show "w \<in> lang (R i j 0)"
     apply(cases)
+    using assms(1) word_run_from_i_j_def apply fastforce
     apply(auto simp add:lang_Rij0 lang_arcs_rexp)
-    using assms word_run_from_i_j_def apply auto
-    by (metis nxts.simps(1) nxts.simps(2) ) +
+    using assms word_run_from_i_j_def intermediate_path_restricted_def apply auto
+    using word_run_sound apply blast
+    by (metis in_mono list.set_intros(1) nxts.simps(1) nxts.simps(2)) +
 qed
 
 
@@ -120,6 +161,7 @@ lemma path_decomposition:"(path_run_from_i_j p i j \<and> intermediate_path_rest
                                                                                       \<and>                 k \<notin> set( p3)
                                                                           )"
   unfolding path_run_from_i_j_def intermediate_path_restricted_def
+  nitpick
   sorry
  
  
@@ -128,9 +170,7 @@ lemma " [i] @  p1 @ [k] @ (concat (intersperse_alt [x,y,z] [k])) @ p3 @ [j] =
   by auto
 
 
-
-
-lemma word_run_from_i_j_trans:"i \<in> S  \<Longrightarrow> j \<in> S \<Longrightarrow>word_run_from_i_j a i j \<Longrightarrow> word_run_from_i_j b j k \<Longrightarrow> word_run_from_i_j (a@b) i k"
+lemma word_run_from_i_j_trans:"word_run_from_i_j a i j \<Longrightarrow> word_run_from_i_j b j k \<Longrightarrow> word_run_from_i_j (a@b) i k"
   unfolding word_run_from_i_j_def
   apply(induction a arbitrary:i)
   apply(auto)
@@ -139,14 +179,19 @@ lemma word_run_from_i_j_trans:"i \<in> S  \<Longrightarrow> j \<in> S \<Longrigh
 lemma start_end_in_path:"word_run_from_i_j u x y  \<Longrightarrow> {x,y} \<subseteq> set (path_of_word u x )" for u x y
     unfolding word_run_from_i_j_def
     apply(induction u arbitrary:x y)
-    by(auto)
- 
+    by (auto simp add: transitions_in_S)
+
+
+fun replicate_list :: "'b list \<Rightarrow> nat \<Rightarrow> 'b list"
+  where
+  "replicate_list lst k = concat (replicate k lst)"
+
 
 
 lemma langRijk: 
-  assumes "i \<in> S  \<and> j \<in> S "
-  shows " w \<in> lang (R i j k) =(word_run_from_i_j w i j \<and>  intermediate_path_restricted (path_of_word w i) k)"
-using assms proof(induction k arbitrary: i j)
+  assumes " k\<le>n "
+  shows " w \<in> lang (R i j k) \<longleftrightarrow> (word_run_from_i_j w i j \<and>  intermediate_path_restricted (path_of_word w i) k)"
+using assms proof(induction k arbitrary: i j w)
   case 0
   then show ?case
     using langR1j0_1 langR1j0_2 by blast
@@ -161,97 +206,87 @@ next
   let ?v = "R (Suc k) (Suc k) k" 
   let ?w = "R (Suc k)    j    k" 
 
-
-
-
  
+  have w_case:"w \<in> lang (R i j (Suc k)) \<longleftrightarrow> w \<in> lang (Plus  ?R' (Times ?u (Times (Star ?v) ?w)))"
+    apply(auto simp add:R_valid_path)
+    using R_valid_path by blast
 
+  have lang_times:"w \<in> lang (Times (R a b k) (R b c k)) \<Longrightarrow> word_run_from_i_j w a c" for a b c w
+    using Suc.IH Suc.prems word_run_from_i_j_trans by fastforce
+
+  have word_run_star:"a \<in> S \<Longrightarrow> w \<in> star (lang (R a a k)) \<Longrightarrow>  word_run_from_i_j w a a" for a w
+  proof -
+    assume "a \<in> S"
+    show "w \<in> star (lang (R a a k)) \<Longrightarrow> word_run_from_i_j w a a"
+      apply(induction rule:star_induct)
+      apply (simp add: \<open>a \<in> S\<close> word_run_from_i_j_def)
+      using Suc.IH Suc.prems Suc_leD word_run_from_i_j_trans by blast
+  qed
+  
+ 
   show ?case 
-  proof(cases "(k+1) \<notin> set (intermediate_path ?p)")
-    case True
+  proof(cases "\<forall>s. s \<in> set (intermediate_path (path_of_word w i)) \<longrightarrow> s \<le>  k")
+    case not_through_k_plus_one:True
 
-    have "w \<in> lang ?R' \<Longrightarrow> (word_run_from_i_j w i j \<and> intermediate_path_restricted (path_of_word w i) (Suc k))"
-    proof -
+    have "w \<in> lang ?R' \<longleftrightarrow> (word_run_from_i_j w i j \<and> intermediate_path_restricted (path_of_word w i) (Suc k))"
+    proof(rule iffI)
       assume "w \<in> lang ?R'"
-
-      then have "w \<in>  lang (Plus ?R' (Times ?u (Times (Star ?v) ?w)))"
-        by(auto)
-
-     then have "w \<in>  lang (Plus ?R' (Times ?u (Times (Star ?v) ?w)))"
-        by(auto)
-
+ 
       show "(word_run_from_i_j w i j \<and> intermediate_path_restricted (path_of_word w i) (Suc k))"
-        sorry
+        by (meson Suc.IH Suc.prems Suc_leD \<open>w \<in> lang (R i j k)\<close> intermediate_path_restricted_def le_SucI)
+    next
+      assume "(word_run_from_i_j w i j \<and> intermediate_path_restricted (path_of_word w i) (Suc k))"
+
+      then have "intermediate_path_restricted (path_of_word w i) k"
+        unfolding intermediate_path_restricted_def
+        using not_through_k_plus_one le_Suc_eq by fastforce
+       
+      then  show "w \<in> lang ?R'"
+        by (simp add: Suc.IH Suc.prems Suc_leD \<open>word_run_from_i_j w i j \<and> intermediate_path_restricted (path_of_word w i) (Suc k)\<close>) 
     qed
 
+    have "(w \<in> lang (R i j (Suc k))) \<Longrightarrow> (word_run_from_i_j w i j \<and> intermediate_path_restricted (path_of_word w i) (Suc k))"
+    proof -
+      assume "(w \<in> lang (R i j (Suc k)))"
+      then show ?thesis
+      proof(cases "(w \<in> lang (R i j k))")
+        case True
+        then show ?thesis
+          by (simp add: \<open>(w \<in> lang (R i j k)) = (word_run_from_i_j w i j \<and> intermediate_path_restricted (path_of_word w i) (Suc k))\<close>) 
+      next
+        case False
 
+        then have "w \<in> lang (Plus  ?R' (Times ?u (Times (Star ?v) ?w)))"
+            using \<open>w \<in> lang (R i j (Suc k))\<close> w_case by blast
 
-    then show ?thesis
-      sorry
-   
+    
+          then have "word_run_from_i_j w i j"
+            apply (simp add: False)
+            using lang_times word_run_star
+            by (smt (verit, best) R_valid_path Suc.IH Suc.prems Suc_leD concE word_run_from_i_j_trans)
+
+ 
+          then have " intermediate_path_restricted (path_of_word w i) (Suc k)"
+            by (simp add: intermediate_path_restricted_def le_SucI not_through_k_plus_one)
+  
+        then show ?thesis
+          by (simp add: \<open>word_run_from_i_j w i j\<close>)
+      qed
+    qed
+
+   then show ?thesis
+     by (metis Rmono Suc_eq_plus1 \<open>(w \<in> lang (R i j k)) = (word_run_from_i_j w i j \<and> intermediate_path_restricted (path_of_word w i) (Suc k))\<close> subset_iff)  
+           
   next
     case False
 
-    let ?u = "R    i    (Suc k) k"
-    let ?v = "R (Suc k) (Suc k) k" 
-    let ?w = "R (Suc k)    j    k"
-
-    have "lang (R i j (Suc k)) =  lang (Plus  ?R' (Times ?u (Times (Star ?v) ?w)))"
-      by (simp add: False)
-
-    let ?p = "path_of_word w i"
-    have " k \<in> set(?p)" 
   
-
-    obtain p1 p2 p3 where "?p = p1 @ p1 @ p3" 
-                            and "path_run_from_i_j p1 i k" and "k \<notin> set(intermediate_path p1)"
-                            and "path_run_from_i_j p2 k k" and "k \<notin> set(intermediate_path p1)"
-                            and "path_run_from_i_j p3 k j" and " k \<notin> set(intermediate_path p3)"
-
-  
-      have "k \<in> set(p)"
-
-  have "word_run_from_i_j w (Suc k) k"
-
-     then show ?thesis 
-       sorry
-  
-  qed
-
-
-qed
-
-
-lemma langRijk: 
-  assumes "i \<in> S  \<and> j \<in> S "
-  shows"  w \<in> lang (R i j k) =  (word_run_from_i_j w i j \<and>  intermediate_path_restricted (path_of_word w i) k)"
-using assms proof(induction k arbitrary: i)
-  case 0
-  then show ?case
-    using langR1j0_1 langR1j0_2 by blast
-
-next
-  case (Suc k)
-
-  show ?case 
-  proof(rule iffI)
-    assume " w \<in> lang (R i j (Suc k))"
-
-    show "word_run_from_i_j w i j \<and> intermediate_path_restricted (path_of_word w i) (Suc k)"  
-      sorry
-
-  next
-    assume "word_run_from_i_j w i j \<and> intermediate_path_restricted (path_of_word w i) (Suc k)"  
-    
-
-  show "    w \<in> lang (R i j (Suc k))"
-    sorry
-
-  qed
-
-qed
  
+     then show ?thesis sorry
+       
 
+   qed
+ qed
 
 
 
@@ -277,8 +312,10 @@ proof -
     by blast
    also have "... = {w.  (\<exists>j \<in> Fin. word_run_from_i_j w 1 j)  }"
      by (metis in_mono start_exist states_subset langRn)
-  also have "...= {w. accepted w }"
-    using accepted_def word_run_from_i_j_def by auto
+   also have "... = {w.  (\<exists>j \<in> Fin.  set w \<subseteq> set sigma \<and> nxts w 1 = j)  }"
+     using start_exist word_run_from_i_j_def by auto
+   also have "...= {w. accepted w }"
+     using accepted_def by auto
   ultimately show ?thesis
     by simp
 qed
